theories/ftlr/Get.v
@@ -1,7 +1,7 @@
 From iris.proofmode Require Import proofmode.
 From iris.program_logic Require Import weakestpre adequacy lifting.
 From stdpp Require Import base.
-From cap_machine Require Export logrel.
+From cap_machine Require Export logrel register_tactics.
 From cap_machine.ftlr Require Export ftlr_base.
 From cap_machine.rules Require Export rules_Get rules_base.
 
@@ -15,20 +15,25 @@ Section fundamental.
   Implicit Types interp : (D).
 
   Lemma get_case (r : leibnizO Reg) (p : Perm)
-        (b e a : Addr) (w : Word) (dst r0 : RegName) (ins: instr) (P:D) :
+        (b e a : Addr) (widc w : Word) (dst r0 : RegName) (ins: instr) (P:D) :
     is_Get ins dst r0 →
-    ftlr_instr r p b e a w ins P.
+    ftlr_instr r p b e a widc w ins P.
   Proof.
     intros Hinstr Hp Hsome i Hbae Hi.
-    iIntros "#IH #Hinv #Hinva #Hreg #[Hread Hwrite] Hown Ha HP Hcls HPC Hmap".
-    rewrite delete_insert_delete.
+    iIntros
+      "#IH #Hinv #Hinva #Hreg #[Hread Hwrite] Hown Ha HP Hcls HPC HIDC Hmap".
+    iInsertList "Hmap" [idc;PC].
+    (* rewrite delete_insert_delete. *)
     rewrite <- Hi in Hinstr. clear Hi.
-    iDestruct ((big_sepM_delete _ _ PC) with "[HPC Hmap]") as "Hmap /=";
-      [apply lookup_insert|rewrite delete_insert_delete;iFrame|]. simpl.
+    (* iDestruct ((big_sepM_delete _ _ PC) with "[HPC Hmap]") as "Hmap /="; *)
+    (*   [apply lookup_insert|rewrite delete_insert_delete;iFrame|]. simpl. *)
     iApply (wp_Get with "[$Ha $Hmap]"); eauto.
     { simplify_map_eq; auto. }
     { rewrite /subseteq /map_subseteq /set_subseteq_instance. intros rr _.
-      apply elem_of_dom. apply lookup_insert_is_Some'; eauto. }
+      apply elem_of_dom. apply lookup_insert_is_Some'; eauto.
+      right.
+      destruct (decide (rr = idc)); subst; simplify_map_eq; auto.
+    }
 
     iIntros "!>" (regs' retv). iDestruct 1 as (HSpec) "[Ha Hmap]".
     destruct HSpec; cycle 1.
@@ -38,15 +43,18 @@ Section fundamental.
     { incrementPC_inv; simplify_map_eq.
       iApply wp_pure_step_later; auto. iMod ("Hcls" with "[HP Ha]");[iExists w;iFrame|iModIntro]. iNext.
       assert (dst <> PC) as HdstPC by (intros ->; simplify_map_eq).
+      (* TODO need to destruct (dst = idc at some point) *)
       iIntros "_".
       simplify_map_eq.
-      iApply ("IH" $! (<[dst := _]> (<[PC := _]> r)) with "[%] [] [Hmap] [$Hown]");
+      iApply ("IH" $! (<[dst := _]> (<[idc := widc]> (<[PC := _]> r))) with "[%] [] [Hmap] [$Hown]");
         try iClear "IH"; eauto.
       { intro. cbn. by repeat (rewrite lookup_insert_is_Some'; right). }
-      iIntros (ri v Hri Hsv). rewrite insert_commute // lookup_insert_ne // in Hsv; [].
+      iIntros (ri v Hri Hsv).
+      (* rewrite insert_commute // lookup_insert_ne // in Hsv; []. *)
       destruct (decide (ri = dst)); simplify_map_eq.
       { repeat rewrite fixpoint_interp1_eq; auto. }
-      { by iApply "Hreg". } rewrite !fixpoint_interp1_eq /=. destruct Hp as [-> | ->];iFrame "Hinv". }
+      { by iApply "Hreg". } rewrite !fixpoint_interp1_eq /=. destruct Hp as
+        [-> | ->]. ;iFrame "Hinv". }
   Qed.
 
 End fundamental.
